# Lemma 4.6
Für $A,A' \in R^{n,m}, B \in R^{m,l}$ und $\lambda \in R$ gelten:
a) $(A^{T})^{T} = A$
b) $(A+ A')^{T}= A^{T} + A'^{T}$
c) $(\lambda \cdot A)^{T}= \lambda \cdot A^{T}$
d) $(A*B)^{T} = B^{T} * A ^{T}$

### Bew
a),b),c) siehe Übung

d)
Für jedes $i \in \{ 1,\dots,n \}, j \in \{ 1,\dots,l \}$ gilt
$[(A*B)^{T}]_{i,j} = [A*B]_{j,i} =\Sum_{k=1}^{m} [A]_{j,k}[B]_{k,i}$
$= \Sum_{k=1}^{m}[A^{T}]_{k,j}[B^{T}]_{i,k}$
$= \Sum_{k=1}^{m}[B^{T}]_{i,k}\cdot [A^{T}]_{k,j}$
$=[B^{T}*A^{T}]_{i,j}$
$\bs$
