# Satz 6.18
FÃ¼r alle $z_{1},z_{2} \in \C$ gilt:
$\exp(z_{1}+z_{2}) = \exp(z_{1}) \exp(z_{2})$ 

Bew:
$\exp(z_{j}) = \Sum_{n=0}^{\infty} \frac{z_{j}^{n}}{n!}, j \in \{  1,2 \}$
$\stackrel{Cauchy-Produkt} \implies \exp(z_{1}) \exp(z_{2}) = \Sum_{n=0}^{\infty} C_{n}$ mit
$C_{n} = \Sum_{k=0}^{n} \frac{z_{1}^{k}}{k!} \frac{z_{2}^{n-k}}{(n-k)!}$
$C_{n} = \frac{1}{n!} \Sum_{k=0}^{n} \frac{n!}{k!(n-k)!} z_{1}^{k} z_{2}^{n-k}$
$= \frac{1}{n!} \Sum_{k=0}^{n} \binom{n}{k} z_{1}^{k} z_{2}^{n-k}$
$= \frac{1}{n!} (z_{1}+z_{2})^{n}$
$\RA \exp(z_{1}) \exp(z_{2}) = \Sum_{n=0}^{\infty} \frac{1}{n!} (z_{1}+z_{2})^{n} = \exp(z_{1}+z_{2})$
$\bs$
