# Satz 6.19
$\F z \in \C, x \in \R$ gilt:
#### 1)
$\exp(z) \neq 0, \exp(-z) = \frac{1}{\exp(z)}$
#### 2)
$\bar{\exp(z)} = \exp(\bar{z})$
#### 3)
$\exp(x) > 0$
#### 4)
$|\exp(ix)| = 1$
#### 5)
$\exp(n) = e^{n} \F n \in \Z$

##### Bem:
In Kapitel 9 wird $a^{x}$ für $a > 0, x \in \C$ definiert. 
Dann wird $\exp(x) = e^{x} \F x \in \C$ gelten

##### Beweis:
1) 
$\exp(z)\exp(-z) = \exp(z - z) = \exp(0) = \exp(1)$
$\RA \exp(z) \neq 0, \exp(-z) = \frac{1}{\exp(z)}$
$\checkmark$
2) 
Sei $S_{m} = \Sum_{n=0}^{\infty} \frac{z^{n}}{n!}$
und $S_{m}^* = \Sum_{n=0}^{\infty} \frac{\bar{z}^{n}}{n!}$

Es gilt $\bar{S_{m}} = S_{m}^*$,
weil $\bar{S_{m}} = \Sum_{n=0}^{ \infty} \frac{z^{n}}{n!} = \Sum_{n=0}^{\infty} \frac{\bar{z}^{n}}{n!} = S_{m}^{*}$
$\exp(\bar{z})$ ist $\limin S_{m}^{*} = \limin conj(s_{m})$
...
3) 
Für $x > 0$ ist $\exp(x) = 1 + x + \frac{x^{2}}{2} + \dots > 0$ 
Für $x < 0$ ist $exp(x) = \frac{1}{\exp(-x)} >0$, da $\exp(-x)>0$

4) 
$conj(\exp(ix)) \stackrel{2)}= \exp(conj(ix)) = \exp(-ix)$ 
$= \frac{1}{\exp(ix)}$ 
$|\exp(ix)|^{2} = \exp(ix) \cdot conj(\exp(ix))$
$= \exp(ix) \cdot \frac{1}{\exp(ix)}$
$= 1$

5) 
a) $n \in \N_{0}$: Induktion
$n = 0 : \exp(0) = 1 = e^{0}$
$n \to n+1$
$\exp(n+1) \stackrel{6.18} = \exp(n)\exp(1) \stackrel{IV}=e ^{n} e = e^{n+1}$

b)
$n \in \Z, n < 0$
$\exp(n) = \exp(- |n|) \stackrel{1)}= \frac{1}{\exp(|n|)} = \frac{1}{e^{|n|}} = e^{-|n|} = e^{n}$
$\bs$
