Seien $f,g: [a,b] \to \R$ integrierbar und $\lambda \in \R$
Dann sind $f+g, \lambda \cdot f: [a,b] \to \R$ integrierbar,
und es gilt:
$(I) \intg_{a}^{b} (f+g)dx = \intg_{a}^{b} f(x)dx + \intg_{a}^{b}g(x)dx$
$(II) \intg_{a}^{b} (\lambda f(x))dx = \lambda \intg_{a}^{b} f(x)dx$
$(III) f\leq g \F x \in [a,b] \RA \intg_{a}^{b}f(x)dx \leq \intg_{a}^{b}g(x)dx$

#### Bew:
Bezeichne $T:= T[a,b]$
$(II)$ Sei $\lambda > 0$
Betrachte $\uint \lambda f = \inf\left( \intg_{a}^{b} \psi ; \psi \in T, \psi \geq \lambda f \right)$
$= \inf\left( \intg_{a}^{b} \lambda \psi*: \psi* \in T, \psi* \geq f \right), \left( \psi*:= \frac{1}{\lambda} \psi\right)$
$\stackrel{L 11.1}= \inf\left( \lambda \intg_{a}^{b} \psi* : \psi* \in T, \psi \geq f \right) = \lambda \inf\left( \intg_{a}^{b} \psi* : \dots \right)$
$= \lambda \uint f(x)dx \stackrel{f\ ibar}= \lambda \intg_{a}^{b} f(x)dx = \lambda \lint f(x)dx$ 
$= sup\left( \intg_{a}^{b}\lambda \varphi : \varphi \in T, \varphi \leq f \right)$
$= sup\left( \intg_{a}^{b} \varphi* : \varphi* \in T, \varphi* \leq \lambda f \right), (\varphi* := \lambda \varphi)$
$= \lint (\lambda f)(x)dx$
$\RA \lambda$ ibar für $\lambda > 0$

Analog für $\lambda < 0$
$\lambda = 0$ trivial
$\checkmark$

$(I)$ siehe skript

$(III)$ Sei $f \leq g$ 
$\intg_{a}^{b} f = \sup\left( \intg_{a}^{b} \psi \in T, \psi \leq f \right) \leq \sup\left( \intg_{a}^{b} \varphi: \varphi \in T, \varphi \leq g \right) = \intg_{a}^{b}(g)$
$\bs$
