# Lemma 4.11
Es seien $A,B \in R^{n,n}$ invertierbar.
Dann gilt:
### a)
$A^{T}$ ist invertierbar mit $(A^{T})^{-1} = (A^{-1})^{T}$ 
(Wir schreiben kurz: $A^{-T}$ f√ºr $(A^{T})^{-1}$)

### b) 
$A * B$ ist invertierbar mit $(A*B)^{-1} = B^{-1} * A^{-1}$

#### Beweis:
a) 
Mithilfe von [[4.11 Lemma 4.6|Lemma 4.6]] folgt:
$(A^{-1})^{T} * A^{T} = (A * A^{-1})^{T} = (I_{n})^{T} = I_{n}$
$=(I_{n})^{T} = (A^{-1} * A)^{T} = A^{T} * (A^{-1})^{T}$
$\RA (A^{-1})^{T} = (A^{T})^{-1}$

b)
Die Aussage gilt in jedem Ring mit Eins ([[3.13 Satz zu Inversen#Satz $III$.13:|Satz 3.13]])
$\bs$
