# Satz 10.14
Sei f,g: $(a,b] \to \R$ diffbar auf $(a,b)$ mit $\Lim_{x \to a+}f(x) = \Lim_{x \to a+}g(x) = 0$
Falls $g'(x) \neq 0 \F x \in (a,b)$ und $q := \Lim_{x \to a+} \frac{f'(x)}{g'(x)} \in \R$, dann
ist $g(x) \neq 0 \F x \in (a,b)$ und 
$\Lim_{x \to a+} \frac{f(x)}{g(x)} = q$

### Bew:
1) Sei $g*(x):= \biggl \{ \begin{matrix} g(x): x \in (a,b]\\ 0, x = a\end{matrix}$

Beh: 
$g(x) \neq 0 \F x \in (a,b)$
Bew:
sonst $\E x_{0} \in (a,b): g(x_{0}) =0$
$\RA g*(x_{0}) = g*(a) = 0 \stackrel{Roll e}\RA g'(\xi) = 0$ für ein $\xi \in (a,b)$ $\contrana$

2.) Nach S.10.13
$\E x_{0} \in (a,x): \frac{f*(x)-f*(a)}{g*(x)-g*(a)} = \frac{f*'(x_{0})}{g*'(x_{0})} = \frac{f'(x_{0})}{g'(x_{0})}$
$= \frac{f(x)}{g(x)}$

Für $x \to a+$ gilt auch $x_{0} \to a+$, also 
$\Lim_{x \to a+} \frac{f(x)}{g(x)} = \Lim_{x_{0} \to a+} \frac{f'(x)}{g'(x)} = q$
$\bs$

### Bem.
Analoges gilt für:
$f,g: [a,b) \to \R, x \to b-$
$f,g: (- \infty, b] \to \R, x \to -\infty$
$f,g : [a,\infty) \to \R, x \to  \infty$

Bsp.:
1) $\Lim_{x \to 1} \frac{x^{\alpha}-1}{\log(x)}$, $\alpha \in \R$
$f(x) = x^{\alpha}-1$, $g(x) = \log(x)$, (beide diffbar auf $(0,\infty)$
$\Lim_{x \to 1} f(x) = 0 = \Lim_{x \to 1} g(x)$
$g'(x) = \frac{1}{x} \neq 0 \F x \in (0,\infty)$
$\Lim_{x \to 1} \frac{f'(x)}{g'(x)} = \Lim_{x \to 1} \frac{\alpha x^{\alpha-1}}{\frac{1}{x}} = \Lim_{x \to 1} \alpha x ^{\alpha} = \alpha$
$\RA \Lim_{x \to 1} \frac{x^{\alpha}-1}{\log(x)} = \alpha$

2) $\Lim_{x \to 0} \frac{x}{\sin(x)}$
// $\sin'(x) = \cos(x) \neq 0 \F x \in \left( -\frac{\pi}{2}, \frac{\pi}{2} \right)$
$= \Lim_{x\to_{0}} \frac{x'}{\sin'(x)} = \Lim_{x \to 0}\frac{1}{\cos(x)} = 1$
