## Satz 6.3
Jeder b-adische Bruch konvergiert in $\mathbb{R}$

Bew:
Betrachte $\Sum_{n = -k}^\infi a_n b^{-n}$ mit $k \in \N_0$
und $a_{j} \in \{ 0, 1,\dots,b-1 \} \F j$ 
FÃ¼r $n \geq -k$ sei $x_{n}=\Sum_{j=-k}^n a_{j}b^{-j}$
z.z.:
$(x_{n})_{n \geq -x}$ ist Cauchy.
Sei $\epsilon > 0$
$\E N \in \N: b^{-N}< \epsilon$ 
Sei $n > m$
$\mid x_{n}-x_{m}\mid = |\Sum_{j=m+1}^na_{j}b^{-j}| \leq (b-1)\Sum_{j=m+1}^n b^{-j}$
da $a_{j} \leq b-1$
$\leq (b-1) b^{-m - 1} \Sum_{k=0}^{m-n-1}b^{-k}$
$\leq (b-1)b^{-m-1} \Sum_{k=0}^{m}b^{-k} = (b-1)b^{-m - 1} \frac{1}{1-b}$
$= b ^{-m} \frac{b-1}{\frac{b(n-1)}{b}} = b ^{-m}$ 
Also 
$|x_{n} - x_{m}|\leq b < \epsilon$ 

Also konvergiert jeder b-adische Bruch gegen eine Reelle Zahl (nach Cauchy)

