# Satz 10.6
Seien $I,J \subseteq \R$ ein offenes Intervall, $f: I \to \R$, g: $J \to \R$, $f(I) \subseteq J$,
f differenzierbar in $x_{0} \in I$, g differenzierbar in $y_{0} = f(x_{0})$.
Dann ist auch $g \circ f: I \to \R$ in $x_{0}$ differenzierbar, und $(g \circ f)(x_{0}) = g'(f(x_{0}))\cdot f'(x_{0})$

#### Bew:
Für $x \in I$ mit $x \neq x_{0}$ betrachte $\frac{(g \circ f)(x) - (g circ f)(x_{0})}{x - x_{0}}$

Sei $g*: J \to \R, g*(y) = \biggl \{ \begin{matrix} \frac{g(y)-g(x)}{y - y_{0}}, y \neq y_{0} \\ g'(y_{0}), y = y_{0}\end{matrix}$

g differenzierbar in $x_{0} \RA g*$ stetig in $y_{0}$
& es gilt $g(y)-g(y_{0}) = g*(y)(y-y_{0})$ für jedes $y \in J$

Also $\Lim_{x \to x_{0}} \frac{g(f(x))-g(f(x_{0}))}{x - x_{0}} = \Lim_{x \to x_{0}} \frac{g*(f(x))(f(x)-f(x_{0}))}{x-x_{0}}$
$= \Lim_{x \to x_{0}}g*(f(x_{0})) \Lim_{x \to x_{0}} \frac{f(x)-f(x_{0})}{x-x_{0}}$
$= g'(f(x_{0}))f'(x_{0})$
$\bs$

#### Bsp:
1)
Für $f: \R \to \R$ diffbar, $a,b \in \R$ betrachte $F(x) := f(ax+b)$
$F'(x)= F'(ax+b) \cdot (ax+b)' = a f'(ax +b)$

2)
$f:(0, \infty) \to \R, f(x):= x^{a}, a \in \R$
$f(x) = \exp(a \log x) \RA f'(x) = \exp'(a \log x) \cdot (a \log x)'$
$= \exp(a \log x) \cdot \frac{a}{x} = a x^{a-1}$

3)
$f: \R \to \R, f(x) = a^{x}, a > 0$
$= \exp(x \log(a))$
$f'(x) = \exp(x \log( a))' \cdot (x \log(a))'$
$= \exp(x \log(a)) \cdot \log(a)$
$= \log(a) \cdot a^{x}$
$\bs$

